Zippy/Zippy/Actions/Zippy_Actions.thy
@@ -7,17 +7,17 @@ theory Zippy_Actions
     Zippy_Identifiers
 begin
 
-ML_file\<open>zippy_paction_mixin_base.ML\<close>
-ML_file\<open>zippy_paction_mixin.ML\<close>
+ML_file\<open>zippy_caction_mixin_base.ML\<close>
+ML_file\<open>zippy_caction_mixin.ML\<close>
 
-ML_file\<open>zippy_paction_queue_mixin_base.ML\<close>
-ML_file\<open>zippy_paction_queue_mixin.ML\<close>
+ML_file\<open>zippy_caction_queue_mixin_base.ML\<close>
+ML_file\<open>zippy_caction_queue_mixin.ML\<close>
 
-ML_file\<open>zippy_presults_mixin_base.ML\<close>
-ML_file\<open>zippy_presults_mixin.ML\<close>
+ML_file\<open>zippy_cresults_mixin_base.ML\<close>
+ML_file\<open>zippy_cresults_mixin.ML\<close>
 
-ML_file\<open>zippy_paction_presults_mixin_base.ML\<close>
-ML_file\<open>zippy_paction_presults_mixin.ML\<close>
+ML_file\<open>zippy_caction_cresults_mixin_base.ML\<close>
+ML_file\<open>zippy_caction_cresults_mixin.ML\<close>
 
 ML_file\<open>zippy_action_metadata.ML\<close>
 ML_file\<open>zippy_action_metadata_mixin_base.ML\<close>
